

# Understanding Analysis Attempt/Solution

pand4monium

November 13, 2025



# Contents

<b>1</b>	<b>The Real Numbers</b>	<b>1</b>
1.2	Some Preliminaries . . . . .	1
1.3	The Axiom of Completeness . . . . .	6



# Chapter 1

## The Real Numbers

### 1.2 Some Preliminaries

#### Exercise 1.2.1

- (a) Prove that  $\sqrt{3}$  is irrational. Does a similar argument work to show  $\sqrt{6}$  is rational?
- (b) Where does the proof break down if we try to prove  $\sqrt{4}$  is irrational?

#### SOLUTION

- (a) AFSOC that  $\sqrt{3}$  is rational, so  $\exists m, n \in \mathbb{Z}$ , such that

$$\sqrt{3} = \frac{m}{n},$$

where  $\frac{m}{n}$  is in the lowest reduced terms. By squaring both sides, we obtain  $3 = (\frac{m}{n})^2 \implies 3n^2 = m^2$ . Now, we know that  $m^2$  is a multiple of 3 and thus  $m$  must also be a multiple of 3. We can then write  $m = 3k$ , deriving

$$\begin{aligned}(\sqrt{3})^2 &= \left(\frac{3k}{n}\right)^2 \\ 3n^2 &= 9k^2 \\ n^2 &= 3k^2\end{aligned}$$

Similar to above, we can conclude that  $n$  is a multiple of 3. However this is a contradiction since  $m, n$  are both multiples of 3 but we assumed that  $\frac{m}{n}$  was in its lowest reduced term. Thus we conclude that  $\sqrt{3}$  is irrational. The same proof for  $\sqrt{3}$  works for  $\sqrt{6}$  as well.

- (b) We cannot conclude that  $\sqrt{4} = \frac{m}{n}$  imply that  $m$  is a multiple of 4, as we have

$$4n^2 = m^2 \implies 2n = m,$$

preventing us from reaching our contradiction that  $m/n$  is not in its lowest terms.

#### Exercise 1.2.2

Show that there is no rational number  $r$  satisfying  $2^r = 3$ .

#### SOLUTION

If  $r = 0$ , then  $2^r = 1 \neq 3$ . Suppose  $r = p/q$  to get  $2^p = 3^q$ , which is not possible as 2 and 3 share no common factors. Hence  $r$  is not rational.

#### Exercise 1.2.3

Decide which of the following represent true statements about the nature of sets. For any that are false, provide a specific example where the statement in question does not hold.

- (a) If  $A_1 \supseteq A_2 \subseteq A_3 \subseteq A_4 \dots$  are all sets containing an infinite number of elements, then the intersections  $\bigcap_{n=1}^{\infty} A_n$  is infinite as well.
- (b) If  $A_1 \supseteq A_2 \subseteq A_3 \subseteq A_4 \dots$  are all finite, nonempty sets of real numbers, then the intersection  $\bigcap_{n=1}^{\infty} A_n$  is finite and non-empty.
- (c)  $A \cap (B \cup C) = (A \cap B) \cup C$ .
- (d)  $A \cap (B \cap C) = (A \cap B) \cap C$ .
- (e)  $A \cap (B \cup C) = (A \cap B) \cup (A \cap C)$ .

**SOLUTION**

- (a) False. Consider  $A_n = \{n, n+1, n+2, \dots\}$ , then  $\bigcap_{n=1}^{\infty} A_n = \emptyset$ .
- (b) True. Since all  $A_n$  are nonempty,  $\exists n \in \mathbb{N}$  such that  $A_n = \{x\}$  for some real  $x$ . Hence  $\bigcap_{n=1}^{\infty} A_n \subseteq \{x\}$  which is empty. Since  $A_1$  is finite,  $\bigcap_{n=1}^{\infty} A_n \subseteq \{x\} \subseteq A_1$  is finite.
- (c) False. If  $A = \emptyset$ , then  $\emptyset = C$
- (d) True. Intersection is associative as evident that both LHS and RHS implies the  $x \in A, B, C$
- (e) True. Drawing a Venn Diagram illustrates this.

**Exercise 1.2.4**

Produce an infinite collection of sets  $A_1, A_2, A_3, \dots$  with the property that every  $A_i$  has an infinite number of elements,  $A_i \cap A_j = \emptyset$  for all  $i \neq j$ , and  $\bigcup_{i=1}^{\infty} A_i = \mathbb{N}$ .

**SOLUTION**

Consider arranging the elements of  $\mathbb{N}$  in a square as such.

1	3	6	10	15	...
2	5	9	14	...	
4	8	13	...		
7	12	...			
11	...				
$\vdots$					

By letting  $A_i$  being the set of all natural numbers in the  $i$ -th row, we have satisfied the above conditions above.

**Exercise 1.2.5**

**(De Morgan's Law)** Let  $A$  and  $B$  be subsets of  $\mathbb{R}$ .

- (a) If  $x \in (A \cap B)^c$ , explain why  $x \in A^c \cup B^c$ . This shows that  $(A \cap B)^c \subseteq A^c \cup B^c$ .
- (b) Prove the reverse inclusion  $(A \cap B)^c \supseteq A^c \cup B^c$ , and conclude that  $(A \cap B)^c = A^c \cup B^c$ .
- (c) Show  $(A \cup B)^c = A^c \cap B^c$  by demonstrating inclusion both ways.

**SOLUTION**

- (a) If  $x \in (A \cap B)^c$ , then  $x \notin A \cap B$ , so  $x \notin A$  or  $x \notin B$ , implying  $x \in A^c$  or  $x \in B^c$ , therefore  $x \in A^c \cup B^c$ .
- (b) If  $x \in A^c \cup B^c$ , then  $x \in A^c$  or  $x \in B^c$ , so  $x \notin A$  and  $x \notin B$ , implying  $x \notin A \cap B$ , therefore  $x \in (A \cap B)^c$ . Since  $(A \cap B)^c \subseteq A^c \cup B^c$  and  $(A \cap B)^c \supseteq A^c \cup B^c$ , we can conclude that both sets are equal.
- (c) To show that  $(A \cap B)^c = A^c \cup B^c$ , we need to demonstrate inclusion both ways.
  - (i) If  $x \in (A \cup B)^c$ , then  $x \notin A \cup B$ , so  $x \notin A$  or  $x \notin B$ , implying  $x \in A^c$  or  $x \in B^c$ , therefore  $x \in A^c \cup B^c$ .

- (ii) If  $x \in A^c \cap B^c$ , then  $x \in A^c$  and  $x \in B^c$ , so  $x \notin A$  and  $x \notin B$ , implying  $x \notin A \cup B$ , which is just  $x \in (A \cup B)^c$ .

**Exercise 1.2.6**

- (a) Verify the triangle inequality in the special case where  $a$  and  $b$  have the same sign.  
 (b) Find an efficient proof for all the cases at once by first demonstrating  $(a + b)^2 \leq (|a| + |b|)^2$ .  
 (c) Prove  $|a - b| \leq |a - c| + |c - d| + |d - b|$  for all  $a, b, c$  and  $d$ .  
 (d) Prove  $||a| - |b|| \leq |a - b|$ . (The unremarkable identity  $a = a - b + b$  may be useful.)

**SOLUTION**

- (a) With both  $a$  and  $b$  having the same sign, then  $|a| + |b| = |a + b|$ , which satisfies  $|a| + |b| \geq |a + b|$ .  
 (b) Note that  $(a + b)^2 \leq (|a| + |b|)^2$  reduces to  $ab \leq |a||b|$ , which is true as LHS can be negative while RHS cannot. Since squaring preserves inequality, this implies that  $|a + b| \leq |a| + |b|$ .  
 (c) Notice that  $a - b = (a - c) + (c - d) + (d - b)$ . Hence by triangle inequality,

$$|a - b| = |(a - c) + (c - d) + (d - b)| \leq |a - c| + |c - d| + |d - b|$$

for all  $a, b, c$  and  $d$ .

- (d) Since  $||a| - |b|| = ||b| - |a||$ , WLOG, we can assume that  $|a| \geq |b|$ . Then

$$||a| - |b|| = |a| - |b| = |(a - b) + b| - |b| \leq |a - b| + |b| - |b| = |a - b|$$

**Exercise 1.2.7**

Given a function  $f$  and a subset  $A$  of its domain, let  $f(A)$  represent the range of  $f$  over the set  $A$ ; that is,  $f(A) = \{f(x) : x \in A\}$ .

- (a) Let  $f(x) = x^2$ . If  $A = [0, 2]$  (the closed interval  $\{x \in \mathbb{R} : 0 \leq x \leq 2\}$ ) and  $B = [1, 4]$ , find  $f(A)$  and  $f(B)$ . Does  $f(A \cap B) = f(A) \cap f(B)$  in this case? Does  $f(A \cup B) = f(A) \cup f(B)$ ?  
 (b) Find two sets  $A$  and  $B$  for which  $f(A \cap B) \neq f(A) \cap f(B)$ .  
 (c) Show that, for an arbitrary function  $g : \mathbb{R} \rightarrow \mathbb{R}$ , it is always true that  $g(A \cap B) \subseteq g(A) \cap g(B)$  for all sets  $A, B \subseteq \mathbb{R}$ .  
 (d) Form and prove a conjecture about the relationship between  $g(A \cup B)$  and  $g(A) \cup g(B)$  for an arbitrary function  $g$ .

**SOLUTION**

- (a) For  $f(x) = x^2$ ,  $f(A) = f([0, 2]) = [0, 4]$  and  $f(B) = f([1, 4]) = [1, 16]$ .

$$f(A \cap B) = f([0, 2] \cap [1, 4]) = f([1, 2]) = [1, 4] = [0, 4] \cap [1, 16] = f([1, 2]) \cap f([2, 4]) = f(A) \cap f(B)$$

$$f(A \cup B) = f([0, 2] \cup [1, 4]) = f([0, 4]) = [0, 16] = [0, 4] \cup [1, 16] = f([0, 2]) \cup f([1, 4]) = f(A) \cup f(B)$$

- (b) Consider  $A = [0, 2]$  and  $B = [-2, 0]$ .  $f(A \cap B) = \{0\}$ , but  $f(A) \cap f(B) = [0, 4]$ .  
 (c) Suppose  $y \in g(A \cap B)$ , then  $\exists x \in A \cap B$  such that  $g(x) = y$ . This implies that  $x \in A$  and  $x \in B$ , so  $x \in A \cap B$ , hence  $y \in g(A \cap B)$ . Note that contrary may not always be true as it is possible for  $x_1 \in A \setminus B$  and  $x_2 \in B \setminus A$  such that  $g(x_1) = g(x_2)$ .  
 (d) I conjecture that  $g(A \cup B) = g(A) \cup g(B)$ . To prove this, we have to show inclusion both ways:  
 (i) Let  $y \in g(A \cup B)$ , then  $\exists x \in A \cup B$  such that  $y = g(x)$ . This implies that  $x \in A$  or  $x \in B$ , so  $y \in g(A)$  or  $y \in g(B)$ , hence  $y \in g(A) \cup g(B)$ .  
 (ii) Let  $y \in g(A) \cup g(B)$ , then  $y \in g(A)$  or  $y \in g(B)$ , implying  $x \in A$  or  $x \in B$  such that  $y = g(x)$ . So  $x \in A \cup B$ , hence  $y \in g(A \cup B)$ .

**Exercise 1.2.8**

Here are two important definitions related to a function  $f : A \rightarrow B$ . The function  $f$  is *one-to-one* (1-1) if  $a_1 \neq a_2$  in  $A$  implies that  $f(a_1) \neq f(a_2)$  in  $B$ . The function  $f$  is *onto* if, given any  $b \in B$ , it is possible to find an element  $a \in A$  for which  $f(a) = b$ . Give an example of each or state that the request is impossible:

(a)  $f : \mathbb{N} \rightarrow \mathbb{N}$  that is 1-1 but not onto.

(b)  $f : \mathbb{N} \rightarrow \mathbb{N}$  that is onto but not 1-1.

(c)  $f : \mathbb{N} \rightarrow \mathbb{Z}$  that is 1-1 and onto.

**SOLUTION**

(a) Let  $f(x) = x + 1$ , which is 1-1 but does not have a solution to  $f(x) = 1$ , hence not onto.

(b) Let  $f(x) = 1$  for  $x = 1$  and  $f(x) = x - 1$  for  $x > 1$ , which is onto but not 1-1 as  $f(1) = f(2) = 1$ .

(c) Let  $f(x) = n/2$  when  $n$  is even and  $f(x) = -\frac{x-1}{2}$  when  $n$  is odd.

**Exercise 1.2.9**

Given a function  $f : D \rightarrow \mathbb{R}$  and a subset  $B \subseteq \mathbb{R}$ , let  $f^{-1}(B)$  be the set of all points from the domain  $D$  that get mapped into  $B$ ; that is  $f^{-1}(B) = \{x \in D : f(x) \in B\}$ . This set is called the *preimage* of  $B$ .

(a) Let  $f(x) = x^2$ . If  $A$  is the closed interval  $[0, 4]$  and  $B$  is the closed interval  $[-1, 1]$ , find  $f^{-1}(A)$  and  $f^{-1}(B)$ . Does  $f^{-1}(A \cap B) = f^{-1}(A) \cap f^{-1}(B)$  in this case? Does  $f^{-1}(A \cup B) = f^{-1}(A) \cup f^{-1}(B)$ ?

(b) The good behaviour of preimages demonstrated in (a) is completely general. Show that for an arbitrary function  $g : \mathbb{R} \rightarrow \mathbb{R}$ , it is always true that  $g^{-1}(A \cap B) = g^{-1}(A) \cap g^{-1}(B)$  and  $g^{-1}(A \cup B) = g^{-1}(A) \cup g^{-1}(B)$  for all sets  $A, B \subseteq \mathbb{R}$ .

**SOLUTION**

(a) For  $f(x) = x^2$ ,  $f^{-1}(A) = [-2, 2]$  and  $f^{-1}(B) = [-1, 1]$ .  $f^{-1}(A \cap B) = f^{-1}([0, 1]) = [-1, 1] = f^{-1}(A) \cap f^{-1}(B)$ . Similarly,  $f^{-1}(A \cup B) = f^{-1}([-1, 4]) = [-2, 2] = f^{-1}(A) \cup f^{-1}(B)$ .

(b) To show that  $g^{-1}(A \cap B) = g^{-1}(A) \cap g^{-1}(B)$ , we have to show inclusion both ways:

(i) Let  $x \in g^{-1}(A \cap B)$ , so  $g(x) \in A \cap B$ , which implies  $g(x) \in A$  and  $g(x) \in B$ . This shows that  $x \in g^{-1}(A)$  and  $x \in g^{-1}(B)$ , hence  $x \in g^{-1}(A) \cap g^{-1}(B)$ .

(ii) Let  $x \in g^{-1}(A) \cap g^{-1}(B)$ , so  $x \in g^{-1}(A)$  and  $x \in g^{-1}(B)$ , then  $g(x) \in A$  and  $g(x) \in B$ . This implies that  $g(x) \in A \cap B$ , so  $x \in g^{-1}(A \cap B)$ .

Showing  $g^{-1}(A \cup B) = g^{-1}(A) \cup g^{-1}(B)$  is obvious using Exercise 1.2.7 (d).

**Exercise 1.2.10**

Decide which of the following are true statements. Provide a short justification for those that are valid and a counterexample for those that are not:

(a) Two real numbers satisfy  $a < b$  if and only if  $a < b + \epsilon$  for every  $\epsilon > 0$ .

(b) Two real numbers satisfy  $a < b$  if  $a < b + \epsilon$  for every  $\epsilon > 0$ .

(c) Two real numbers satisfy  $a \leq b$  if and only if  $a < b + \epsilon$  for every  $\epsilon > 0$ .

**SOLUTION**

(a) False. Consider the case where  $a < b + \epsilon$  is true but  $a = b$ .

(b) False. Same reasoning as above.

(c) True. Firstly suppose  $a < b + \epsilon$  for all  $\epsilon > 0$ . We need to show this implies  $a \leq b$ . We either have  $a \leq b$  or  $a > b$ . However,  $a > b$  is not possible as this implies there exists an  $\epsilon$  small enough such that  $a > b + \epsilon$ . Secondly, suppose  $a \leq b$ . It is obvious that  $a < b + \epsilon$  for all  $\epsilon > 0$ .



**Exercise 1.2.11**

Form the logical negation of each claim. One trivial way to do this is to simply add "It is not the case that..." in front of each assertion. To make this more interesting, fashion the negation into a positive statement that avoids using the word "not" altogether. In each case, make an intuitive guess as to whether the claim or its negation is the true statement.

- (a) For all real numbers satisfying  $a < b$ , there exists an  $n \in \mathbb{N}$  such that  $a + 1/n < b$ .
- (b) There exists a real number  $x > 0$  such that  $x < 1/n$  for all  $n \in \mathbb{N}$ .
- (c) Between every two distinct real numbers there is a rational number.

**SOLUTION**

- (a) For all  $n \in \mathbb{N}$ , there exists  $a, b \in \mathbb{R}$  such that  $a + 1/n < b$ . [FALSE]
- (b) For all real number  $x > 0$ , there exists an  $n \in \mathbb{N}$  such that  $x \geq 1/n$ . [TRUE]
- (c) There exists two real numbers  $a < b$  such that if  $r < b$  then  $r < a$  for all  $r \in \mathbb{Q}$ . [FALSE]

**Exercise 1.2.12**

Let  $y_1 = 6$ , and for each  $n \in \mathbb{N}$  define  $y_{n+1} = (2y_n - 6)/3$ .

- (a) Use induction to prove that the sequence satisfies  $y_n > -6$  for all  $n \in \mathbb{N}$ .
- (b) Use another induction argument to show the sequence  $(y_1, y_2, y_3, \dots)$  is decreasing.

**SOLUTION**

- (a) For  $n = 1$ ,  $y_1 = 6 > -6$  (Base Case). Suppose  $y_n > -6$  for some  $n \in \mathbb{N}$ .

$$y_{n+1} = \frac{2y_n - 6}{3} > \frac{2(-6) - 6}{3} = -6$$

Hence, by induction,  $y_n > -6$  for all  $n \in \mathbb{N}$ .

- (b) Suppose  $y_{n+1} < y_n$ . The base case works as  $y_2 = 2 < 6 = y_1$ . Then,

$$\begin{aligned} y_{n+1} < y_n &\implies 2y_{n+1} - 6 < 2y_n - 6 \\ &\implies \frac{2y_{n+1} - 6}{3} < \frac{2y_n - 6}{3} \\ &\implies y_{n+2} < y_{n+1} \end{aligned}$$

Thus,  $y_{n+1} < y_n$  is true for all  $n \in \mathbb{N}$ .

**Exercise 1.2.13**

For this exercise, assume Exercise 1.2.5 has been successfully completed.

- (a) Show how induction can be used to conclude that

$$(A_1 \cup A_2 \cup \dots \cup A_n)^c = A_1^c \cap A_2^c \cap \dots \cap A_n^c$$

for any finite  $n \in \mathbb{N}$ .

- (b) It is tempting to appeal to induction to conclude

$$\left( \bigcup_{i=1}^{\infty} A_i \right)^c = \bigcap_{i=1}^{\infty} A_i^c$$

but induction does not apply here. Induction is used to prove that a particular statement holds for every value of  $n \in \mathbb{N}$ , but this does not imply the validity of the infinite case. To illustrate this point, find an example of a collection of sets  $B_1, B_2, B_3, \dots$  where  $\bigcap_{i=1}^n B_i \neq \emptyset$  is true for every  $n \in \mathbb{N}$ , but  $\bigcap_{i=1}^{\infty} B_i \neq \emptyset$  fails.

- (c) Nevertheless, the infinite version of De Morgan's Law stated in (b) is a valid statement. Provide a proof that does not use induction.

**SOLUTION**

- (a) Using Exercise 1.2.5 as the base case. Suppose  $(A_1 \cup \dots \cup A_n)^c = A_1^c \cap \dots \cap A_n^c$  is true. Using associative law on the  $n + 1$ c case,

$$\begin{aligned} ((A_1 \cup \dots \cup A_n) \cup A_{n+1})^c &= (A_1 \cup \dots \cup A_n)^c \cap A_{n+1}^c \\ &= (A_1^c \cap \dots \cap A_n^c) \cap A_{n+1}^c \\ &= A_1^c \cap \dots \cap A_n^c \cap A_{n+1}^c \end{aligned}$$

- (b) Consider  $B_1 = \{1, 2, \dots\}$ ,  $B_2 = \{2, 3, \dots\}$ ,  $B_n = \{x : x \in \mathbb{N} \cap [n, \infty)\}$ .
- (c) To prove the infinite version of De Morgan's Law, we need to show inclusion both ways.
- (i) Suppose  $x \in (\bigcup_{i=1}^{\infty} A_i)^c$ , then  $x \notin \bigcup_{i=1}^{\infty} A_i$ . This implies that  $x \notin A_i \ \forall i \in \mathbb{N}$ , so  $x \in A_i^c \ \forall i \in \mathbb{N}$ . Hence  $x \in \bigcap_{i=1}^{\infty} A_i^c$ .
- (ii) Suppose  $x \in \bigcap_{i=1}^{\infty} A_i^c$ , then  $x \in A_i^c \ \forall i \in \mathbb{N}$ , so  $x \notin A_i \ \forall i \in \mathbb{N}$ . This implies that  $x \notin \bigcup_{i=1}^{\infty} A_i$ , hence  $x \in (\bigcup_{i=1}^{\infty} A_i)^c$ .

## 1.3 The Axiom of Completeness

**Exercise 1.3.1**

- (a) Write a formal definition in the style of Definition 1.3.2 for the *infimum* or *greatest lower bound* of a set.
- (b) Now, state and prove a version of Lemma 1.3.8 for greatest lower bound.

**SOLUTION**

- (a) A real number  $i$  is the *greatest upper bound* for a set  $A \subseteq \mathbb{R}$  if it meets the following two criteria:
- (i)  $i$  is a lower bound of  $A$ ;
- (ii) if  $b$  is any lower bound for  $A$ , then  $i \geq b$ .
- (b) Assume  $i \in \mathbb{R}$  is a lower bound for a set  $A \subseteq \mathbb{R}$ . Then  $i = \inf A$  if and only if, for every choice of  $\epsilon > 0$ , there  $\exists a \in A$  satisfying  $i + \epsilon > a$ .

PROOF Rephrasing the lemma gives us: Given that  $i$  is a lower bound,  $i$  is the greatest lower bound if and only if any number greater than  $i$  is not a lower bound.

- (i) Suppose  $i = \inf A$  and consider  $i + \epsilon$  for an arbitrarily chosen  $\epsilon > 0$ . Since  $i + \epsilon > i$ , part (ii) of the definition implies that  $i + \epsilon$  is not a lower bound for  $A$ . If this is the case, then there must be some element  $a \in A$  such that  $i + \epsilon > a$ .
- (ii) Conversely, assume  $i$  is a lower bound with the property that for any  $\epsilon > 0$ ,  $i + \epsilon$  is not a lower bound of  $A$ . Note that this implies that if  $b$  is any number more than  $i$ , then  $b$  is not an upperbound. Since we have argued that any larger number than  $i$  cannot be a lower bound, if  $b$  is some other upper bound for  $A$ , then  $i \geq b$ .

**Exercise 1.3.2**

Give an example of each of the following, or state that the request is impossible.

- (a) A set  $B$  with  $\inf B \geq \sup B$ .
- (b) A finite set that contains its infimum but not its supremum.
- (c) A bounded subset of  $\mathbb{Q}$  that contains its supremum but not its infimum.

**SOLUTION**

- (a) Possible. Consider the set  $0$ , where  $\inf\{0\} = \sup\{0\} = 0$ .
- (b) Not possible as all finite sets must contain its supremum and infimum.
- (c) Possible. Consider  $A = \{r \in \mathbb{Q} \mid 1 < r \leq 2\}$ .

**Exercise 1.3.3**

- (a) Let  $A$  be nonempty and bounded below, and define  $B = \{b \in \mathbb{R} : b \text{ is a lower bound for } A\}$ . Show that  $\sup B = \inf A$ .
- (b) Use (a) to explain why there is no need to assert that greatest lower bounds exist as part of the Axiom of Completeness.

**SOLUTION**

- (a) By definition,  $\sup B$  is the greatest lower bound for  $A$ , meaning it equals  $\inf A$ .
- (b) Part (a) proves the greatest lower bound exists using the least upper bound.

**Exercise 1.3.4**

Let  $A_1, A_2, A_3, \dots$  be a collection of nonempty sets, each of which is bounded above.

- (a) Find a formula for  $\sup(A_1 \cup A_2)$ . Extend this to  $\sup(\bigcup_{k=1}^n A_k)$ .
- (b) Consider  $\sup(\bigcup_{k=1}^{\infty} A_k)$ . Does the formula in (a) extend to the infinite case?

**SOLUTION**

- (a)  $\sup(A_1 \cup A_2) = \sup\{\sup A_1, \sup A_2\}$  and  $\sup(\bigcup_{k=1}^n A_k) = \sup\{\sup A_k \mid k = 1, \dots, n\}$
- (b) This formula does not extend to infinity. Consider  $A_k = [k, k+1]$ , where  $\bigcup_{k=1}^{\infty} A_k$  is unbounded.

**Exercise 1.3.5**

As in Example 1.3.7, let  $A \subseteq \mathbb{R}$  be nonempty and bounded above, and let  $c \in \mathbb{R}$ . This time define the set  $cA = \{ca : a \in A\}$ .

- (a) If  $c \geq 0$ , show that  $\sup(cA) = c \sup A$ .
- (b) Postulate a similar type of statement for  $\sup(cA)$  for the case  $c < 0$ .

**SOLUTION**

- (a) The case of  $c = 0$  is trivial as it implies that  $cA = \{0\}$ . Hence  $\sup(cA) = c \sup A = 0$ .  
For  $c > 0$ , we need to show that  $c \sup A$  is the lowest upper bound. Assume  $c > 0$ . Let  $s = c \sup A$ . Suppose  $ca > s$ , then  $a > \sup A$  which is impossible, meaning that  $s$  is an upper bound on  $cA$ . Now suppose  $s'$  is an upper bound on  $cA$  and  $s' < s$ . Then  $s'/c < s/c = \sup A$ , meaning  $s'/c$  cannot bound  $A$ . Hence there  $\exists a \in A$  such that  $s'/c < a$ , meaning  $s' > ca$ , thus  $s'$  cannot be an upper bound on  $cA$ , so  $s = c \sup A$  is the least upper bound.
- (b)  $\sup(cA) = c \inf A$  for  $c < 0$

**Exercise 1.3.6**

Given sets  $A$  and  $B$ , define  $A + B = \{a + b : a \in A \text{ and } b \in B\}$ . Follow these steps to prove that if  $A$  and  $B$  are nonempty and bounded above then  $\sup(A + B) = \sup A + \sup B$ .

- (a) Let  $s = \sup A$  and  $t = \sup B$ . Show  $s + t$  is an upper bound for  $A + B$ .
- (b) Now let  $u$  be an arbitrary upper bound for  $A + B$ , and temporarily fix  $a \in A$ . Show  $t \leq u + a$ .
- (c) Finally, show  $\sup(A + B) = s + t$ .
- (d) Construct another proof of this same fact using Lemma 1.3.8.

**SOLUTION**

- (a) By definition of supremum,  $a \leq s$  and  $b \leq t$ . Adding both equations give  $a + b \leq s + t$ , hence  $s + t$  is an upper bound.
- (b) Since  $a + b \leq u$  implies  $b \leq u - a$ ,  $u - a$  is an upper bound on  $b$ , meaning it is greater or equal to the least upper bound of  $b$ , giving  $t \leq u - a$ .
- (c) From (a), we have shown that  $s + t$  is an upper bound for  $A + B$ , hence it is sufficient to show that  $s + t$  is the least upper bound.
- Let  $u = \sup(A + B)$ , from (b) we have  $t \leq u - a$  and  $s \leq u - b$ . Adding and rearranging gives  $a + b \leq 2u - s - t$ . Since  $2u - s - t$  is an upper bound on  $A + B$ , it must be greater or equal to the least upper bound, giving  $u \leq 2u - s - t$ , implying  $s + t \leq u$ . Since  $u$  is the least upper bound,  $s + t$  must equal  $u$ .
- (d) Showing  $s + t - \epsilon$  is not an upper bound for any  $\epsilon > 0$  proves that it is the least upper bound by Lemma 1.3.8. Rearranging gives  $(s - \epsilon/2) + (t - \epsilon/2)$  we know  $\exists a > (s - \epsilon/2)$  and  $b > (t - \epsilon/2)$ , therefore  $a + b > s + t - \epsilon$ , meaning  $s + t$  cannot be made smaller and thus is the least upper bound.